Completeness for POR! plus some reorganizing

SymPaths.v
@@ -186,7 +186,155 @@ Qed.
 (*
   Framing corresponds to accumulated substitutions with different initial states
   when working with (this style of) traces. We will see how hard/easy that is to incorporate
+
+  Turns out we can make do without
 *)
+
+(* This is not quite confluence, but kind of step-wise *)
+Theorem diamond_property: forall s1 s2 s1' s2' t e1 e2,
+    red__S (t, <{s1 || s2}>) (t :: e1, <{s1' || s2}>) ->
+    red__S (t, <{s1 || s2}>) (t :: e2, <{s1 || s2'}>) ->
+    red__S (t :: e1, <{s1' || s2}>) ((t :: e1) :: e2, <{s1' || s2'}>) /\
+    red__S (t :: e2, <{s1 || s2'}>) ((t :: e2) :: e1, <{s1' || s2'}>)
+.
+Proof.
+  split.
+  - dependent destruction H0. dependent destruction H1;
+      inversion x0; inversion x; subst.
+    + dependent destruction H0;
+        apply cons_neq' in x; contradiction.
+    + dependent destruction H0;
+        apply context_injective in H5; try discriminate; try assumption; symmetry in H5;
+        [ apply SIf_true_disjoint in H5
+        | apply SIf_false_disjoint in H5
+        | apply SSeq_disjoint in H5
+        | apply SPar_right_disjoint in H5
+        | apply SPar_left_disjoint in H5];
+        contradiction.
+    + dependent destruction H0;
+        try (apply cons_neq' in x; contradiction);
+        try (apply ctx_red_intro with (C := fun s => SPar s1' (C s));
+             [constructor | constructor; assumption]).
+  - dependent destruction H. dependent destruction H0;
+      inversion x0; inversion x; subst.
+    + dependent destruction H;
+        apply cons_neq' in x; contradiction.
+    + dependent destruction H;
+        try (apply cons_neq' in x; contradiction);
+        try (apply ctx_red_intro with (C := fun s => SPar (C s) s2');
+             [constructor | constructor; assumption]).
+    + dependent destruction H;
+        apply context_injective in H6; try assumption; apply symmetry in H6;
+        [ discriminate
+        | apply SIf_true_disjoint in H6
+        | apply SIf_false_disjoint in H6
+        | apply SSeq_disjoint in H6
+        | apply SPar_right_disjoint in H6
+        | apply SPar_left_disjoint in H6];
+        contradiction.
+Qed.
+
+Lemma equiv_step: forall s t1 s' t1' t2,
+    t1 ~ t2 -> red__S (t1, s) (t1', s') ->
+    exists t2', red__S (t2, s) (t2', s') /\ t1' ~ t2'.
+Proof.
+  intros. inversion H0; subst. inversion H4; subst; eexists; split;
+    try (constructor; [constructor | assumption]);
+    try (apply path_equiv_extend);
+    assumption.
+Qed.
+
+Theorem equiv_star: forall s t1 s' t1' t2,
+    t1 ~ t2 -> red_star__S (t1, s) (t1', s') ->
+    exists t2', red_star__S (t2, s) (t2', s') /\ t1' ~ t2'.
+Proof.
+  intros. dependent induction H0.
+  - exists t2. split; [constructor | assumption].
+  - destruct y. edestruct (IHclos_refl_trans_n1 s t1 s0 t) as [t2' [IHcomp IHequiv]];
+      try assumption; try reflexivity.
+    destruct (equiv_step _ _ _ _ _ IHequiv H1) as [t2_final [comp_final equiv_final]].
+    exists t2_final. split.
+    + econstructor. apply comp_final. apply IHcomp.
+    + assumption.
+Qed.
+
+Definition selection_function: Type := forall t, {t' : trace__S | t ~ t'}.
+Definition select (f:selection_function) (t: trace__S) := proj1_sig (f t).
+
+Definition id_select: selection_function.
+  intro. econstructor. reflexivity.
+Defined.
+
+Variant head_red__POR (f: selection_function): relation (trace__S * Stmt) :=
+  | POR_intro: forall s s' t t',
+      head_red__S (select f t, s) (t', s') ->
+      head_red__POR f (t, s) (t', s').
+
+Definition red__POR f := context_red (head_red__POR f).
+Definition red_star__POR f := clos_refl_trans_n1 _ (red__POR f).
+
+Ltac solve_equivs := repeat (
+      match goal with
+      | _ : _ |- ?t ~ ?t => reflexivity
+      | H : ?t ~ ?t' |- ?t' ~ ?t => symmetry in H; assumption
+      | H1 : ?t1 ~ ?t2, H2 : ?t2 ~ ?t3 |- ?t1 ~ ?t3 => transitivity t2; assumption
+      | H1 : ?t2 ~ ?t1, H2 : ?t2 ~ ?t3 |- ?t1 ~ ?t3 => symmetry in H1
+      | _ : _ |- (?t :: _) ~ (?t' :: _) => apply path_equiv_extend
+      (* dealing with selection functions*)
+      | _ : _ |- ?t' ~ select ?f ?t => unfold select; destruct (f t); simpl
+      | _ : _ |- select ?f ?t ~ ?t' => unfold select; destruct (f t); simpl
+      | H : ?T |- ?T => apply H
+      | _ => fail
+      end).
+
+Theorem correctness__POR: forall f s0 t0 s t,
+    red_star__POR f (t0, s0) (t, s) ->
+    exists t', red_star__S (t0, s0) (t', s) /\ t ~ t'.
+Proof.
+  intros. dependent induction H.
+  - exists t. split; constructor.
+  - destruct y. destruct (IHclos_refl_trans_n1 s0 t0 s1 t1) as [t' [IHcomp IHequiv]];
+      try reflexivity.
+    dependent destruction H. dependent destruction H.
+    specialize (equiv_step (C s2) (select f t1) (C s') t t'). intros.
+    destruct H2 as [t2 [equiv_step Hequiv]].
+    + solve_equivs.
+    + constructor; assumption.
+    + eexists. split.
+      * econstructor.
+        ** apply equiv_step.
+        ** assumption.
+      * assumption.
+Qed.
+
+Lemma completeness_step__POR: forall f t0 t0' s0 t s,
+    t0 ~ t0' ->
+    red__S (t0, s0) (t, s) ->
+    exists t', red__POR f (t0', s0) (t', s) /\ t ~ t'.
+Proof.
+  intros. inversion H0; inversion H4; subst; eexists; split;
+    try (constructor; [repeat constructor | assumption]);
+    solve_equivs.
+Qed.
+
+Theorem completeness__POR: forall f t0 s0 t s,
+    red_star__S (t0, s0) (t, s) ->
+    exists t', red_star__POR f (t0, s0) (t', s) /\ t ~ t'.
+Proof.
+  intros. dependent induction H.
+  - exists t. split; constructor.
+  - destruct y. destruct (IHclos_refl_trans_n1 t0 s0 t1 s1) as [t' [IHcomp IHequiv]];
+      try reflexivity.
+    destruct (completeness_step__POR f t1 t' s1 t s) as [t_step [comp_step equiv_step]];
+      try assumption; solve_equivs.
+    exists t_step. split.
+    + econstructor.
+      * apply comp_step.
+      * apply IHcomp.
+    + assumption.
+Qed.
+
+(** * Dynamic Logic (section 4)*)
 
 Inductive DL : Type :=
   | DLExpr (b: Bexpr)
